refactoring in dependent classes

examples/enumSTProofs.v
@@ -15,13 +15,11 @@ Require Import enumProofs. (* TODO change *)
 Set Bullet Behavior "Strict Subproofs".
 
 
+(* Set Typeclasses Debug. *)
+(* QuickChickDebug Debug On. *)
+
 Derive EnumSizedSuchThat for (fun n => le m n).
 
-
-(* Example with two IH *)
-
-Set Typeclasses Debug.
-QuickChickDebug Debug On.
 
 Inductive goodTree : nat -> tree nat  -> Prop :=
 | GL : forall a, goodTree 0 (Leaf nat a)
@@ -44,46 +42,26 @@ Proof. derive_sound (). Qed.
 Instance DecOptgoodTree_list_complete n t : DecOptCompletePos (goodTree n t).
 Proof. derive_complete (). Qed.
 
-
 Derive EnumSizedSuchThat for (fun t => goodTree k t).
-(* Why is it taking so much time? *) 
 
-Lemma enumerate_SizeMonotonic (A : Type) (l : seq (E (option A))) :
-  l \subset SizeMonotonic ->
-  SizeMonotonic (enumerate l).
-Proof.
-  unfold enumerate. 
-  assert (Datatypes.length l = Datatypes.length l)%coq_nat by reflexivity.  
-  revert H.
-  generalize (Datatypes.length l) at 2 3 4.
-  intros n. revert l. induction n; intros l Heq Hsub.
-  - simpl. now eauto with typeclass_instances.
-  - simpl.
-    eapply bindMonotonicStrong; eauto with typeclass_instances.
-    
-    intros x1 Hin. eapply Enumerators.semChoose in Hin; eauto. simpl in *. 
-    
-    destruct (Enumerators.pickDrop_exists l x1). simpl in *. now ssromega.
-    destruct H. destruct H. destruct H0. destruct H1.
 
-    rewrite H.
+Inductive tree1 :=
+| Leaf1 : tree1
+| Node1 : nat -> tree1 -> tree1 -> tree1.
 
-    eapply bindMonotonicStrong; eauto with typeclass_instances.
-    
-    intros a Hin'.
 
-    destruct a; eauto with typeclass_instances. 
+Inductive bst : nat -> nat -> tree1 -> Prop :=
+| BstLeaf : forall n1 n2, bst n1 n2 Leaf1
+| BstNode : forall min max n t1 t2,
+    le min max -> le min n -> le n max ->
+    bst min n t1 -> bst n max t2 ->
+    bst min max (Node1 n t1 t2).
 
-    eapply returnGenSizeMonotonic; eauto with typeclass_instances.
 
-    assert (Heq' : (n.+1 - 1) = n). { ssromega. }
+Derive DecOpt for (bst min max t).
 
-    rewrite Heq'. eapply IHn. 
 
-    now ssromega.
-
-    eapply subset_trans. eassumption. eassumption.
-Qed.
+Derive EnumSizedSuchThat for (fun t => bst min max t).
 
 
 Ltac2 simpl_minus_enumSizeST (_ : unit) :=
@@ -91,55 +69,6 @@ Ltac2 simpl_minus_enumSizeST (_ : unit) :=
 
 Ltac2 simpl_enumSizeST (_ : unit) :=
   unfold enumSizeST; simpl_minus_enumSizeST (). 
-
-Ltac2 rec enumST_size_mon (ih : ident) :=
-  first
-    [ (* ret *)
-      eapply returnGenSizeMonotonic;
-      now eauto with typeclass_instances
-    | (* bindOpt *)
-      eapply bindMonotonicOpt >
-      [ now eauto with typeclass_instances
-      | first
-          [ (* for calls to enum in params *)
-            now eauto with typeclass_instances 
-          | (* for call to existing enum instances. XXX not sure why typeclass resulotion doesn't work *)
-            eapply sizedSizeMonotonic; now eauto with typeclass_instances 
-          | (* for recursive calls *)
-             let ih' := Control.hyp ih in 
-            eapply $ih' ]
-      | let x := Fresh.in_goal (id_of_string "x") in
-        intros $x; enumST_size_mon ih
-      ]
-    | (* bind *)
-      eapply bindMonotonic >
-      [ now eauto with typeclass_instances
-      | first
-          [ (* for calls to enum in params *)
-            now eauto with typeclass_instances 
-          | (* for call to existing enum instances. XXX not sure why typeclass resulotion doesn't work *)
-            eapply sizedSizeMonotonic; now eauto with typeclass_instances 
-          | (* for recursive calls *)
-             let ih' := Control.hyp ih in 
-            eapply $ih' ]
-      | let x := Fresh.in_goal (id_of_string "x") in
-        intros $x; enumST_size_mon ih
-      ]
-    | (* input matching *)
-      match! goal with
-      | [ |- SizeMonotonic (match ?p with _ => _ end) ] =>
-        destruct $p; enumST_size_mon ih
-      end
-    | ()
-    ].
-
-Ltac2 rec enumsST_size_mon (t : constr) (ih : ident) :=
-  first
-    [ now eapply (@list_subset_nil (E (option $t)))
-    | eapply (@list_subset_cons (E (option $t))) > 
-      [ now enumST_size_mon @ih
-      | enumsST_size_mon t ih ] ]. 
-
 
 Ltac2 revert_params (inst : constr) :=
   match Constr.Unsafe.kind inst with
@@ -157,218 +86,13 @@ Ltac2 intro_params (inst : constr) :=
   | _ => () 
   end.
 
-Ltac2 derive_enumST_SizeMonotonic (_ : unit) :=
-  let s := Fresh.in_goal (id_of_string "s") in
-  let ihs := Fresh.in_goal (id_of_string "Ihs") in
-  let si := Fresh.in_goal (id_of_string "si") in
-  intro $s;
-  let s' := Control.hyp s in 
-
-  match! goal with
-  | [ |- SizeMonotonic (@enumSizeST ?typ ?pred ?inst _) ] =>   
-    simpl_enumSizeST (); generalize $s' at 1; revert_params inst;
-    induction $s' as [ | $s $ihs ]; intro_params inst; intros $si;
-       eapply enumerate_SizeMonotonic; 
-       now enumsST_size_mon typ @IHs
-  end.
-
-Instance EnumSizedSuchThatgoodTree_SizeMonotonic n :
-  forall s, SizeMonotonic (@enumSizeST _ _ (@EnumSizedSuchThatgoodTree n) s).
-Proof. derive_enumST_SizeMonotonic (). Qed.
-
-Lemma enumerate_correct_size_opt {A} (lst : list (E (option A))) s :
-  semProdSizeOpt (enumerate lst) s <--> \bigcup_(x in lst) (semProdSizeOpt x s).
-Proof.
-  assert (Hc := enumerate_correct_size lst s).
-  intros x. destruct (Hc (Some x)) as [H1 H2].
-  split.
-  - intros Hin. simpl in *.
-
-    assert (Hin' : ((fun u : option A => u) :&: semEnumSize (enumerate lst) s) (Some x)).
-    { split; eauto. }
-    
-    eapply Hc in Hin'. destruct Hin'. inv H. inv H3.
-    eexists. split; eauto.
-
-  - intros Hin. simpl in *.
-    
-    assert (Hin' : (\bigcup_(x in lst) ((fun u : option A => u) :&: semEnumSize x s)) (Some x)).
-    { inv Hin. inv H. eexists; split; eauto. split; eauto. }
-    
-    eapply Hc in Hin'. destruct Hin'. eassumption.
-Qed.       
-
-Lemma enumerate_correct_opt {A} (lst : list (E (option A))) :
-  semProdOpt (enumerate lst) <--> \bigcup_(x in lst) (semProdOpt x).
-Proof.
-  split; intros H.
-  - inv H. inv H0.
-    assert (Hin : semProdSizeOpt (enumerate lst) x a).
-    { eassumption. }
-    eapply (@enumerate_correct_size_opt A) in Hin.
-    inv Hin. inv H0.
-    eexists. split; eauto. eexists. split; eauto.
-  - destruct H. destruct H. destruct H0. destruct H0.
-    assert (Hin :  (\bigcup_(x in lst) (semProdSizeOpt x x0)) a).
-    { eexists. split; eauto. }
-    eapply (@enumerate_correct_size_opt A) in Hin.
-    eexists. split; eauto. 
-Qed.       
-
-
-Lemma semReturnSizeOpt {G : Type -> Type} {H : Producer G} {_ : ProducerSemantics}
-      (A : Type) (x : A) (size : nat) :
-  semProdSizeOpt (ret (Some x)) size <--> [set x].
-Proof.
-  intros x1; simpl; split; intros Hin.
-  - unfold semProdSizeOpt, somes in *.
-    eapply semReturnSize in Hin. inv Hin. reflexivity.
-
-  - unfold semProdSizeOpt, somes in *.
-    eapply semReturnSize. inv Hin. reflexivity.
-Qed. 
-
-Lemma semReturnSizeOpt_None {G : Type -> Type}
-      {H : Producer G} {_ : ProducerSemantics}
-      (A : Type) (size : nat) :
-  semProdSizeOpt (ret None) size <--> @set0 A.
-Proof.
-  intros x1; simpl; split; intros Hin.
-  - unfold semProdOpt, somes in *.
-    eapply semReturnSize in Hin. inv Hin.
-  - inv Hin.
-Qed. 
-
-Lemma semReturnOpt {G : Type -> Type} {H : Producer G} {_ : ProducerSemantics}
-      (A : Type) (x : A) :
-  semProdOpt (ret (Some x)) <--> [set x].
-Proof.
-  intros x1; simpl; split; intros Hin.
-  - unfold semProdOpt, somes in *.
-    eapply semReturn in Hin. inv Hin. reflexivity.
-    
-  - unfold semProdOpt, somes in *.
-    eapply semReturn. inv Hin. reflexivity.
-Qed. 
-
-
-Lemma semReturnOpt_None {G : Type -> Type}
-      {H : Producer G} {_ : ProducerSemantics}
-      (A : Type):
-  semProdOpt (ret None) <--> @set0 A.
-Proof.
-  intros x1; simpl; split; intros Hin.
-  - unfold semProdOpt, somes in *.
-    eapply semReturn in Hin. inv Hin.
-  - inv Hin.
-Qed. 
-
-Lemma semOptBind {G : Type -> Type} {H : Producer G} {_ : ProducerSemantics}
-      A B (g : G A) (f : A -> G (option B)) :
-  SizeMonotonic g ->
-  (forall a : A, SizeMonotonic (f a)) ->
-  semProdOpt (bind g f) <-->
-  \bigcup_(a in semProd g) semProdOpt (f a).
-Proof.
-  intros Hs Hsf.
-  unfold semProdOpt.
-  rewrite semBindSizeMonotonic; eauto.
-
-  split.
-  - intros Hin. inv Hin. inv H1.
-    eexists. split; eauto.
-
-  - intros Hin. inv Hin. inv H1.
-    eexists. split; eauto.
-Qed. 
-
-Lemma semOptBindSize {G : Type -> Type} {H : Producer G} {_ : ProducerSemantics}
-      A B (g : G A) (f : A -> G (option B)) size :
-  semProdSizeOpt (bind g f) size <-->
-  \bigcup_(a in semProdSize g size) semProdSizeOpt (f a) size.
-Proof.
-  unfold semProdSizeOpt.
-  rewrite semBindSize; eauto.
-
-  split.
-  - intros Hin. inv Hin. inv H1.
-    eexists. split; eauto.
-
-  - intros Hin. inv Hin. inv H1.
-    eexists. split; eauto.
-Qed. 
-
-Lemma semOptBindOpt {G : Type -> Type} {H : Producer G} {_ : ProducerSemantics}
-      A B (g : G (option A)) (f : A -> G (option B)) :
-  SizeMonotonic g ->
-  (forall a : A, SizeMonotonic (f a)) ->
-  semProdOpt (bindOpt g f) <-->
-  \bigcup_(a in semProdOpt g) semProdOpt (f a).
-Proof.
-  intros Hs Hsf.
-  unfold bindOpt. rewrite semOptBind; eauto.
-  
-  - split. 
-    + intros Hin. inv Hin. inv H1.
-      destruct x. eexists. split; eauto.
-      eapply semReturnOpt_None in H3. inv H3.
-
-    + intros Hin. inv Hin. inv H1.
-      eexists. split; eauto.
-
-  - intros a; destruct a; eauto with typeclass_instances.
-Qed.
-
-Lemma semOptBindOptSize {G : Type -> Type} {H : Producer G} {_ : ProducerSemantics}
-      A B (g : G (option A)) (f : A -> G (option B)) size :
-  semProdSizeOpt (bindOpt g f) size <-->
-  \bigcup_(a in semProdSizeOpt g size) semProdSizeOpt (f a) size.
-Proof.
-  unfold bindOpt. rewrite semOptBindSize; eauto.
-  
-  - split. 
-    + intros Hin. inv Hin. inv H1.
-      destruct x. eexists. split; eauto.
-      eapply semReturnSizeOpt_None in H3. inv H3.
-
-    + intros Hin. inv Hin. inv H1.
-      eexists. split; eauto.
-Qed. 
-
-
+(*** Sized monotonic *) 
 
 Ltac2 rec enums_sized_mon (ih : ident) :=
   first
     [ now eapply incl_bigcup_list_nil
     | eapply incl_bigcup_compat_list > [ | enums_sized_mon ih ] ].
 
-Lemma semBindOptSizeOpt_subset_compat
-      (G : Type -> Type) (PG : Producer G)
-      { _ : ProducerSemantics }
-      (A B : Type) (g g' : G (option A)) (f f' : A -> G (option B)) s : 
-  semProdSizeOpt g s \subset semProdSizeOpt g' s ->
-  (forall (x : A),
-      semProdSizeOpt (f x) s \subset semProdSizeOpt (f' x) s) ->
-  semProdSizeOpt (bindOpt g f) s \subset semProdSizeOpt (bindOpt g' f') s.
-Proof.
-  intros Hyp1 Hyp2.
-  rewrite !semOptBindOptSize.
-  eapply incl_bigcup_compat; eauto.
-Qed. 
-
-Lemma semBindSizeOpt_subset_compat
-      (G : Type -> Type) (PG : Producer G)
-      { _ : ProducerSemantics }
-      (A B : Type) (g g' : G A) (f f' : A -> G (option B)) s : 
-  semProdSize g s \subset semProdSize g' s ->
-  (forall (x : A),
-      semProdSizeOpt (f x) s \subset semProdSizeOpt (f' x) s) ->
-  semProdSizeOpt (bind g f) s \subset semProdSizeOpt (bind g' f') s.
-Proof.
-  intros Hyp1 Hyp2.
-  rewrite !semOptBindSize.
-  eapply incl_bigcup_compat; eauto.
-Qed.
 
 
 Ltac2 rec enumST_sized_mon (ih : ident) :=
@@ -377,14 +101,14 @@ Ltac2 rec enumST_sized_mon (ih : ident) :=
       now eapply subset_refl
     | (* dec matching *)
       match! goal with
-      | [ |- semProdSizeOpt (match decOpt ?s1 with _ => _ end) _ \subset
+      | [ |- semProdSizeOpt (match @decOpt ?p ?i ?s1 with _ => _ end) _ \subset
              semProdSizeOpt (match decOpt ?s2 with _ => _ end) _ ] =>
         let hdec := Fresh.in_goal (id_of_string "Hdec") in 
-        destruct (decOpt $s1) eqn:$hdec >
+        destruct (@decOpt $p $i $s1) eqn:$hdec >
         [ ((erewrite CheckerProofs.mon > [ | | eassumption ]) > [ enumST_sized_mon ih | ssromega ])
-        | rewrite semReturnSizeOpt_None; now eapply sub0set ]
+        | rewrite (@semReturnSizeOpt_None E _ ProducerSemanticsEnum); now eapply sub0set ]
       end
-    | (* input matching *)
+     | (* input matching *) 
       match! goal with
       | [ |- semProdSizeOpt (match ?p with _ => _ end) _ \subset _ ] =>
         destruct $p; enumST_sized_mon ih
@@ -404,22 +128,23 @@ Ltac2 rec enumST_sized_mon (ih : ident) :=
       | let x := Fresh.in_goal (id_of_string "x") in
         intros $x; enumST_sized_mon ih
       ]
+    | ()
     ].
 
 Ltac2 rec find_enum (ih : ident) :=
   first
     [ now eapply incl_bigcup_list_nil
-    | eapply incl_bigcup_compat_list > [ now (enumST_sized_mon ih)  | find_enum ih ]
+    | eapply incl_bigcup_compat_list > [ (enumST_sized_mon ih)  | find_enum ih ]
     | eapply incl_bigcup_list_tl; find_enum ih
     ].
 
 Ltac2 base_case_size_mon (s2 : constr) :=
   destruct $s2 > 
-  [ now eapply subset_refl | rewrite !enumerate_correct_size_opt; now find_enum @dummy ]. 
+  [ now eapply subset_refl | rewrite !enumerate_correct_size_opt; find_enum @dummy ]. 
 
 Ltac2 ind_case_sized_mon (s2 : constr) (ih : ident) :=
   destruct $s2 > 
-  [ now ssromega |  rewrite !enumerate_correct_size_opt; now find_enum ih ]. 
+  [ now ssromega |  rewrite !enumerate_correct_size_opt; find_enum ih ]. 
 
 Ltac2 derive_enumST_SizedMonotonic (_ : unit) :=
   match! goal with
@@ -447,125 +172,338 @@ Ltac2 derive_enumST_SizedMonotonic (_ : unit) :=
 
 Instance EnumSizedSuchThatgoodTree_SizedMonotonic n :
   SizedMonotonicOpt (@enumSizeST _ _ (@EnumSizedSuchThatgoodTree n)).
-Proof. now derive_enumST_SizedMonotonic (). Qed. 
+Proof. derive_enumST_SizedMonotonic (). Qed.
+
+Instance EnumSizedSuchThatle_SizedMonotonic n :
+  SizedMonotonicOpt (@enumSizeST _ _ (@EnumSizedSuchThatle n)).
+Proof. derive_enumST_SizedMonotonic (). Qed.
+
+Instance EnumSizedSuchThatbst_SizedMonotonic min max :
+  SizedMonotonicOpt (@enumSizeST _ _ (@EnumSizedSuchThatbst min max)).
+Proof. derive_enumST_SizedMonotonic (). Qed.  
+
+(* Size Monotonicity *) 
+ 
+Ltac2 rec enumST_size_mon (ih : ident) :=
+  first
+    [ (* ret *)
+      eapply returnGenSizeMonotonicOpt;
+      now eauto with typeclass_instances
+    | (* bindOpt *)
+      eapply bindOptMonotonicOpt >
+      [ now eauto with typeclass_instances
+      | first
+          [ (* for calls to enum in params *)
+            now eauto with typeclass_instances 
+          | (* for call to existing enum instances. XXX not sure why typeclass resulotion doesn't work *)
+            eapply sizedSizeMonotonicOpt; now eauto with typeclass_instances 
+          | (* for recursive calls *)
+             let ih' := Control.hyp ih in 
+            eapply $ih' ]
+      | let x := Fresh.in_goal (id_of_string "x") in
+        intros $x; enumST_size_mon ih
+      ]
+    | (* bind *)
+      eapply bindMonotonicOpt >
+      [ now eauto with typeclass_instances
+      | first
+          [ (* for calls to enum in params *)
+            now eauto with typeclass_instances 
+          | (* for call to existing enum instances. XXX not sure why typeclass resulotion doesn't work *)
+            eapply sizedSizeMonotonic; now eauto with typeclass_instances 
+          | (* for recursive calls *)
+             let ih' := Control.hyp ih in 
+            eapply $ih' ]
+      | let x := Fresh.in_goal (id_of_string "x") in
+        intros $x; enumST_size_mon ih
+      ]
+    | (* input/dec matching *)
+      match! goal with
+      | [ |- SizeMonotonicOpt (match ?p with _ => _ end) ] =>
+        destruct $p; enumST_size_mon ih
+      end
+    | ()
+    ].
+
+Ltac2 rec enumsST_size_mon (t : constr) (ih : ident) :=
+  first
+    [ now eapply (@list_subset_nil (E (option $t)))
+    | eapply (@list_subset_cons (E (option $t))) > 
+      [ enumST_size_mon @ih
+      | enumsST_size_mon t ih ] ]. 
+
+
+Ltac2 derive_enumST_SizeMonotonic (_ : unit) :=
+  let s := Fresh.in_goal (id_of_string "s") in
+  let ihs := Fresh.in_goal (id_of_string "Ihs") in
+  let si := Fresh.in_goal (id_of_string "si") in
+  intro $s;
+  let s' := Control.hyp s in 
+
+  match! goal with
+  | [ |- SizeMonotonicOpt (@enumSizeST ?typ ?pred ?inst _) ] =>   
+    simpl_enumSizeST (); generalize $s' at 1; revert_params inst;
+    induction $s' as [ | $s $ihs ]; intro_params inst; intros $si;
+    eapply enumerate_SizeMonotonicOpt; enumsST_size_mon typ @IHs
+  end.
+
+Instance EnumSizedSuchThatgoodTree_SizeMonotonic n :
+  forall s, SizeMonotonicOpt (@enumSizeST _ _ (@EnumSizedSuchThatgoodTree n) s).
+Proof. derive_enumST_SizeMonotonic (). Qed.
+
+Instance EnumSizedSuchThatle_SizeMonotonic n :
+  forall s, SizeMonotonicOpt (@enumSizeST _ _ (@EnumSizedSuchThatle n) s).
+Proof. derive_enumST_SizeMonotonic (). Qed.
+
+Instance EnumSizedSuchThatbst_SizeMonotonic min max :
+  forall s, SizeMonotonicOpt (@enumSizeST _ _ (@EnumSizedSuchThatbst min max) s).
+Proof. derive_enumST_SizeMonotonic (). Qed.
 
 
 Class CorrectSizedST {A : Type} (P : A -> Prop) {G} `{Producer G} (g : nat -> G (option A)) :=
-  { corrST : [ set x | exists s, semProdOpt (g s) x ]  <-->  [set x : A | P x ] }.
+  { corrST : [ set x | exists s, semProdOpt (g s) x ]  <-->  P }.
 
+Class CorrectST {A : Type} (P : A -> Prop) {G} `{Producer G} (g : G (option A)) :=
+  { corr : semProdOpt g  <-->  P  }.
 
-Instance EnumSizedSuchThatgoodTree_SizedMonotonic n :
-  CorrectSizedST (goodTree n) (@enumSizeST _ _ (@EnumSizedSuchThatgoodTree n)).
+Instance size_CorrectST {A : Type} (P : A -> Prop) {G} {PG : Producer G}
+         {PS: @ProducerSemantics G PG} (g : nat -> G (option A))
+         {Hm1 : forall s, SizeMonotonicOpt (g s)}
+         {Hm2 : SizedMonotonicOpt g}
+         {_ : CorrectSizedST P g} : CorrectST P (sized g).
 Proof.
-  match! goal with
-  | [ |- CorrectSizedST _ (@enumSizeST ?typ ?pred ?inst) ] =>
-    assert (Henum := @enumerate_correct_opt $typ);
-
-    let x := Fresh.in_goal (id_of_string "x") in
-        
+  inv H. constructor.
+  intros x. split; intros Hin.
+  - eapply corrST0.
+    inv Hin. inv H. eapply semSizedSize in H1.
+    eexists. eexists; split; eauto.
+  - eapply corrST0 in Hin. inv Hin. inv H. inv H0.
+    eexists (max x0 x1). split; eauto. eapply semSizedSize.
+    eapply Hm1 > [ | eapply Hm2 > [ | eassumption ]]; ssromega. 
+Qed.
     
-    simpl_enumSizeST (); (); split; intros $x; split >
-      [ (* sound *) | (* complete *) admit ]
+Ltac2 get_ty (e : constr) :=
+  match Constr.Unsafe.kind e with
+  | Constr.Unsafe.Lambda b app =>
+    match Constr.Unsafe.kind app with
+    | Constr.Unsafe.App ty args  => ty
+    | _ => Control.throw (Tactic_failure (Some (Message.of_string ("Expecting an application"))))
+    end
+  | _ => Control.throw (Tactic_failure (Some (Message.of_string ("Expecting a function"))))
+  end.
+
+(* TODO duplicate *)
+
+Ltac2 make_prod (bs : constr array) (c : constr) :=
+  let bs := Array.map (fun b => let t := Constr.type b in
+                                Constr.Binder.make (Some (constr_to_ident b)) t) bs in
+  
+  Array.fold_left (fun t b => Constr.Unsafe.make (Constr.Unsafe.Prod b t)) c bs.
+
+
+(* To derive monotonicity inside the correctness proof *)
+Ltac2 mon_expr (tapp : constr) (inst : constr) :=
+  match! goal with
+  | [ |- CorrectSizedST _ ?f ] =>
+    match Constr.Unsafe.kind f with
+    | Constr.Unsafe.Lambda b app =>
+      match Constr.Unsafe.kind app with
+      | Constr.Unsafe.App aux args =>
+
+        let len := Int.sub (Array.length args) 2 in
+        let inps := Array.sub args 2 len in
+
+        let args' (s1 : constr) (s2 : constr) (offs : int) :=
+            let ind := Array.mapi (fun i _ => Constr.Unsafe.make (Constr.Unsafe.Rel (Int.add i offs))) inps in
+            let a := Array.make 2 s1 in
+            Array.set a 1 s2; Array.append a ind
+        in
+
+        let aux_app s1 s2 := Constr.Unsafe.make (Constr.Unsafe.App aux (args' s1 s2 1)) in
+
+        let dummy_app s1 s2 :=
+            let args' := Array.copy args in
+            let _ := Array.set args' 0 s1 in
+            let _ := Array.set args' 1 s1 in
+            Constr.Unsafe.make (Constr.Unsafe.App aux args')
+        in
+
+        let dummy_term := constr:(SizeMonotonicOpt (ltac2:(let t := dummy_app '0 '0 in exact $t))) in
+
+        let make_term s1 s2 :=
+            match Constr.Unsafe.kind dummy_term with
+            | Constr.Unsafe.App mon margs =>
+              let margs' := Array.copy margs in
+              Array.set margs' 3 (aux_app s1 s2);
+              make_prod inps (Constr.Unsafe.make (Constr.Unsafe.App mon margs'))
+            | _ => Control.throw (Tactic_failure (Some (Message.of_string ("Expecting an application"))))
+            end
+        in 
+
+        assert (Hmon : forall (_s1 _s2 : nat), ltac2:(let s1 := Control.hyp @_s1 in
+                                                      let s2 := Control.hyp @_s2 in
+                                                      let t := make_term s1 s2  in exact $t)) >
+        [  let s := Fresh.in_goal (id_of_string "s") in 
+           let si := Fresh.in_goal (id_of_string "si") in 
+           let ihs := Fresh.in_goal (id_of_string "IHs") in 
+           intros $si $s;
+           let s' := Control.hyp s in revert $si;
+           induction $s' as [ | $s $ihs ]; intros $si;
+           Array.iter (fun _ => intro) inps; eapply enumerate_SizeMonotonicOpt; now enumsST_size_mon tapp ihs
+        | ]
+
+      | _ => Control.throw (Tactic_failure (Some (Message.of_string ("Expecting an application"))))
+      end
+    | _ => Control.throw (Tactic_failure (Some (Message.of_string ("Expecting a function"))))
+    end
+end.
+
+
+Ltac2 find_size_mon_inst (_ : unit) :=
+  first [ now eauto with typeclass_instances
+        | eapply sizedSizeMonotonicOpt; now eauto with typeclass_instances
+        | eapply sizedSizeMonotonic; now eauto with typeclass_instances ].
+
+
+
+Ltac2 rec sound_enum (ty : constr) (ih : ident) :=    
+  match! goal with
+  (* match decOpt *) 
+  | [ h : semProdOpt (match @decOpt ?p ?i ?s with _ => _ end) ?x |- _ ] =>
+    let hdec := Fresh.in_goal (id_of_string "Hdec") in 
+    let b := Fresh.in_goal (id_of_string "b") in 
+    destruct (@decOpt $p $i $s) as [ $b | ] eqn:$hdec > [ | now eapply (@semReturnOpt_None E _ _) in $h; inv $h ];
+    let b' := Control.hyp b in                                                            
+    destruct $b' > [ | now eapply (@semReturnOpt_None E _ _) in $h; inv $h ];
+    eapply (@sound $p) in Hdec > [ | now eauto with typeclass_instances ]; sound_enum ty ih
+
+ (* match input *) 
+  | [ h : semProdOpt (match ?n with _ => _ end) ?x |- _ ] =>
+    destruct $n; try (now eapply (@semReturnOpt_None E _ _) in $h; inv $h); sound_enum ty ih
+  | (* return *)
+    [ h : semProdOpt (returnEnum _) _ |- _ ] =>
+    eapply (@semReturnOpt E _ _) in $h; inv $h;  now eauto 20 using $ty
+  | (* bindOpt *)
+    [ h : semProdOpt (bindOpt _ _) _ |- _ ] =>
+    eapply (@semOptBindOpt E _ _) in $h >
+                                     [ let h' := Control.hyp h in
+                                       (* let x := Fresh.in_goal (id_of_string "_x") in *)
+                                       (* let hin1 := Fresh.in_goal (id_of_string "_Hin1") in *)
+                                       (* let hin2 := Fresh.in_goal (id_of_string "_Hin2") in *)
+                                       (* XXX there seems to be a bug in fresh, and it fails to freshen after a while.
+                                         P     icking ? for now *) 
+                                       destruct $h' as [? [$h ?]];
+                                       let ih' := Control.hyp ih in 
+                                       first [ eapply $ih' in $h | eapply corr in $h (* TODO test and fix *) ];
+                                       sound_enum ty ih
+                                     | find_size_mon_inst ()
+                                     | intro; now enumST_size_mon @Hmon ]
+
+
+  | (* bind *)
+    [ h : semProdOpt (bindEnum _ _) _ |- _ ] =>
+    eapply (@semOptBind E _ _) in $h >
+                                  [ let h' := Control.hyp h in
+                                    destruct $h' as [? [? ?]]; sound_enum ty ih
+                                  | find_size_mon_inst ()
+                                  | intro; now enumST_size_mon @Hmon ]
+
+  | [ |- _ ] => ()
+  end.
+
+Ltac2 rec sound_enums (ty : constr) (ih : ident) :=
+  match! goal with
+  | [ h : (\bigcup_(x in (seq_In (_ :: _))) _) _ |- _ ] =>
+    eapply in_bigcup_list_cons in $h;
+    let h' := Control.hyp h in
+    destruct $h' as [ | ] > [ sound_enum ty ih | sound_enums ty ih  ]
+  | [ h : (\bigcup_(x in seq_In nil) _) _ |- _ ] =>
+    apply bigcup_nil_set0 in $h; inv $h
+  end. 
+
+Ltac2 derive_sound_enumST (ty : constr) (inst : constr) :=
+  let s := Fresh.in_goal (id_of_string "s") in
+  let si := Fresh.in_goal (id_of_string "si") in
+  let ihs := Fresh.in_goal (id_of_string "ihs") in
+  let hgen := Fresh.in_goal (id_of_string "Hgen") in
+  intros [$s $hgen]; revert $hgen;
+
+  let s' := Control.hyp s in
+
+  match! goal with
+    [ |- semProdOpt _ ?x -> _ ] => 
+    (generalize $s' at 1; revert_params inst; revert x; induction $s' as [ | $s $ihs]; intro; intro_params inst;
+     intros $si $hgen;
+     eapply &Henum in $hgen) > [ sound_enums ty ihs | sound_enums ty ihs  ]
   end.
 
 
-  Ltac2 sound_enumST (_ : unit) :=
-    let s := Fresh.in_goal (id_of_string "s") in
-    let si := Fresh.in_goal (id_of_string "si") in
-    let ihs := Fresh.in_goal (id_of_string "ihs") in
-    let hgen := Fresh.in_goal (id_of_string "Hgen") in
-    intros [$s $hgen]; revert $hgen;
+Ltac2 derive_enumST_Correct (_ : unit) := 
+  match! goal with
+  | [ |- CorrectSizedST _ (@enumSizeST ?tapp ?pred ?inst) ] =>
+    assert (Henum := @enumerate_correct_opt $tapp);
+      
+    simpl_enumSizeST ();
 
-    let s' := Control.hyp s in
+    (* derive monotonicity *) 
+    mon_expr tapp inst;
 
-    generalize $s' at 1; induction $s' as [ | $s $ihs]; intros $si $hgen;
-    eapply &Henum in $hgen.
+    let ty := get_ty pred in
+    let x := Fresh.in_goal (id_of_string "x") in
+    split; intros $x; split >
+      [ derive_sound_enumST ty inst | (* complete *) admit ]
+  end.
+
+Instance EnumSizedSuchThatgoodTree_Correct n :
+  CorrectSizedST (goodTree n) (@enumSizeST _ _ (@EnumSizedSuchThatgoodTree n)).
+Proof. derive_enumST_Correct (). Admitted. 
+
+Instance EnumSizedSuchThatle_Correct n :
+  CorrectSizedST (le n) (@enumSizeST _ _ (@EnumSizedSuchThatle n)).
+Proof. derive_enumST_Correct (). Admitted.
+
+Instance EnumSizedSuchThatbst_SizeMonotonic min max :
+  CorrectSizedST (bst min max) (@enumSizeST _ _ (@EnumSizedSuchThatbst min max)).
+Proof.
+  derive_enumST_Correct ().
   
-  sound_enumST ().
-  
-  rewrite Henum in Hgen. 
-  erewrite enumerate_correct_opt in Hgen.
+       eapply (@semOptBindOpt E _ _) in H.
 
-  Focus 2. 
-  revert $hgen. 
-  
-  now derive_enumST_SizedMonotonic (). Qed. 
+       destruct H as [? [H ? ] ].
 
-           
-Inductive tree1 :=
-| Leaf1 : tree1
-| Node1 : nat -> tree1 -> tree1 -> tree1.
-
-
-Inductive bst : nat -> nat -> tree1 -> Prop :=
-| BstLeaf : forall n1 n2, bst n1 n2 Leaf1
-| BstNode : forall min max n t1 t2,
-    le min max -> le min n -> le n max ->
-    bst min n t1 -> bst n max t2 ->
-    bst min max (Node1 n t1 t2).
-
-
-Derive DecOpt for (bst min max t).
-
-
-Derive EnumSizedSuchThat for (fun t => bst min max t).
+       Set Printing All. 
+       eapply (@corr in H. 
+       @semProdOpt E ProducerEnum nat
+        (@sizedEnum (option nat) (@enumSizeST nat (fun n : nat => le min n) (EnumSizedSuchThatle min))) x0
+       admit.
+       now find_size_mon_inst ().
+       intro; now enumST_size_mon @Hmon.
+       
+       
+$h >
+                                     [ let h' := Control.hyp h in
+                                       (* let x := Fresh.in_goal (id_of_string "_x") in *)
+                                       (* let hin1 := Fresh.in_goal (id_of_string "_Hin1") in *)
+                                       (* let hin2 := Fresh.in_goal (id_of_string "_Hin2") in *)
+                                       (* XXX there seems to be a bug in fresh, and it fails to freshen after a while.
+                                         P     icking ? for now *) 
+                                       destruct $h' as [? [$h ?]];
+                                       let ih' := Control.hyp ih in 
+                                       first [ eapply $ih' in $h | eapply corr in $h (* TODO test and fix *) ];
+                                       sound_enum ty ih
+                                     | find_size_mon_inst ()
+                                     | intro; now enumST_size_mon @Hmon ]
 
 
-Definition test min_ max_:=
-  (let
-   fix aux_arb init_size size0 (min_ : nat) (max_ : nat) : E (Coq.Init.Datatypes.option (tree1)) :=
-     match size0 with
-     | O => enumerate (Coq.Lists.List.cons
-                         (@returnEnum (option (tree1)) (@Some (tree1) (@Leaf1))) Coq.Lists.List.nil)
-     | S size' =>
-         enumerate
-           (Coq.Lists.List.cons (@returnEnum (option (tree1)) (@Some (tree1) (@Leaf1)))
-              (Coq.Lists.List.cons
-                 match @decOpt (@le min_ max_) _ init_size as s with
-                 | Some res_b =>
-                     match res_b with
-                     | true =>
-                         @bindEnumOpt nat tree1 (@enumSuchThat _ (fun n => @le min_ n) _)
-                           (fun n =>
-                            match @decOpt (@le n max_) _ init_size as s return E (Coq.Init.Datatypes.option (tree1)) with
-                            | Some res_b =>
-                                match res_b with
-                                | true =>
-                                    @bindEnumOpt tree1 tree1 (aux_arb init_size size' min_ n)
-                                      (fun t1 =>
-                                      @bindEnumOpt tree1 tree1 (aux_arb init_size size' n max_)
-                                         (fun t2 => @returnEnum (option (tree1)) (@Some (tree1) (@Node1 n t1 t2))))
-                                | false => @returnEnum (option (tree1)) (@None (tree1))
-                                end
-                            | None => @returnEnum (option (tree1)) (@None (tree1))
-                            end)
-                     | false => @returnEnum (option (tree1)) (@None (tree1))
-                     end
-                 | None => @returnEnum (option (tree1)) (@None (tree1))
-                 end Coq.Lists.List.nil))
-     end in
- fun size0 => aux_arb size0 size0 min_ max_).
+Admitted.
+ derive_enumST_SizeMonotonic (). Qed.
 
-  let
-    fix aux_arb (init_size size0 min_0 max_0 : nat) {struct size0} : E (option tree1) :=
-    match size0 with
-    | 0 => enumerate [:: returnEnum (Some Leaf1)]
-    | size'.+1 =>
-      enumerate
-        [:: returnEnum (Some Leaf1);
-        match decOpt init_size with
-        | Some true =>
-          bindEnumOpt (enumST [eta le min_0])
-                      (fun n : nat =>
-                         match decOpt init_size with
-                         | Some true =>
-                           bindEnumOpt (aux_arb init_size size' min_0 n)
-                                       (fun t1 : tree1 =>
-                                          bindEnumOpt (aux_arb init_size size' n max_0)
-                                                      (fun t2 : tree1 => returnEnum (Some (Node1 n t1 t2))))
-                         | _ => returnEnum None
-                         end)
-        | _ => returnEnum None
-        end]
-    end in
-  fun size0 : nat => aux_arb size0 size0 min_ max_.
+
+
+       
+
+
+
+Instance EnumSizedSuchThatgoodTree_Correct n :
+  CorrectSizedST (goodTree n) (@enumSizeST _ _ (@EnumSizedSuchThatgoodTree n)).
+Proof. derive_enumST_Correct (). Admitted. 
