src/Enumerators.v
@@ -355,3 +355,133 @@ Proof.
     eapply (@enumerate_correct_size A) in Hin.
     inv Hin. split; eauto. eexists. split; eauto. 
 Qed.   
+
+Lemma enumerate_SizeMonotonic (A : Type) (l : list (E (option A))) :
+  l \subset SizeMonotonic ->
+  SizeMonotonic (enumerate l).
+Proof.
+  unfold enumerate. 
+  assert (Datatypes.length l = Datatypes.length l)%coq_nat by reflexivity.  
+  revert H.
+  generalize (Datatypes.length l) at 2 3 4.
+  intros n. revert l. induction n; intros l Heq Hsub.
+  - simpl. now eauto with typeclass_instances.
+  - simpl.
+    eapply bindMonotonicStrong; eauto with typeclass_instances.
+    
+    intros x1 Hin. eapply Enumerators.semChoose in Hin; eauto. simpl in *. 
+    
+    destruct (Enumerators.pickDrop_exists l x1). simpl in *. now ssromega.
+    destruct H. destruct H. destruct H0. destruct H1.
+
+    rewrite H.
+
+    eapply bindMonotonicStrong; eauto with typeclass_instances.
+    
+    intros a Hin'.
+
+    destruct a; eauto with typeclass_instances. 
+
+    eapply returnGenSizeMonotonic; eauto with typeclass_instances.
+
+    assert (Heq' : (n.+1 - 1) = n). { ssromega. }
+
+    rewrite Heq'. eapply IHn. 
+
+    now ssromega.
+
+    eapply subset_trans. eassumption. eassumption.
+Qed.
+
+
+Lemma enumerate_SizeMonotonicOpt (A : Type) (l : list (E (option A))) :
+  l \subset SizeMonotonicOpt ->
+  SizeMonotonicOpt (enumerate l).
+Proof.
+  unfold enumerate. 
+  assert (Datatypes.length l = Datatypes.length l)%coq_nat by reflexivity.  
+  revert H.
+  generalize (Datatypes.length l) at 2 3 4.
+  intros n. revert l. induction n; intros l Heq Hsub.
+  - simpl. now eauto with typeclass_instances.
+  - simpl.
+    intros s1 s2 Hleq.
+    
+    erewrite !semOptBindSize; eauto with typeclass_instances.
+
+    intros x Hin. inv Hin. inv H.
+    eapply Enumerators.semChooseSize in H0; eauto. simpl in *. 
+
+    destruct (Enumerators.pickDrop_exists l x0). simpl in *. now ssromega.
+    destruct H2. destruct H2. destruct H3. destruct H4.
+
+    rewrite H2 in H1. 
+
+    assert (Hbind := @semBindSize E _ _).
+    simpl in *. eapply Hbind in H1.
+
+
+    destruct H1 as [a [Hina Hin2]].
+
+    destruct a.
+
+    + exists x0. split.
+
+      eapply Enumerators.semChooseSize. simpl. now ssromega.
+      simpl. now ssromega.
+
+      rewrite H2.
+
+      eapply Hbind. exists (Some a). split.
+      
+      eapply Hsub in Hina. simpl in Hina. eassumption.
+      eassumption. ssromega.
+
+      assert (Hret := @semReturnSize E _ _).
+      eapply Hret. eapply Hret in Hin2. eassumption.
+
+    + replace (n.+1 - 1) with n in * by ssromega.
+      admit.
+      (* TODO need lemma about pickDrop *) 
+Admitted.
+
+
+Lemma enumerate_correct_size_opt {A} (lst : list (E (option A))) s :
+  semProdSizeOpt (enumerate lst) s <--> \bigcup_(x in lst) (semProdSizeOpt x s).
+Proof.
+  assert (Hc := enumerate_correct_size lst s).
+  intros x. destruct (Hc (Some x)) as [H1 H2].
+  split.
+  - intros Hin. simpl in *.
+
+    assert (Hin' : ((fun u : option A => u) :&: semEnumSize (enumerate lst) s) (Some x)).
+    { split; eauto. }
+    
+    eapply Hc in Hin'. destruct Hin'. inv H. inv H3.
+    eexists. split; eauto.
+
+  - intros Hin. simpl in *.
+    
+    assert (Hin' : (\bigcup_(x in lst) ((fun u : option A => u) :&: semEnumSize x s)) (Some x)).
+    { inv Hin. inv H. eexists; split; eauto. split; eauto. }
+    
+    eapply Hc in Hin'. destruct Hin'. eassumption.
+Qed.       
+
+Lemma enumerate_correct_opt {A} (lst : list (E (option A))) :
+  semProdOpt (enumerate lst) <--> \bigcup_(x in lst) (semProdOpt x).
+Proof.
+  split; intros H.
+  - inv H. inv H0.
+    assert (Hin : semProdSizeOpt (enumerate lst) x a).
+    { eassumption. }
+    eapply (@enumerate_correct_size_opt A) in Hin.
+    inv Hin. inv H3.
+    eexists. split; eauto. eexists. split; eauto.
+  - destruct H. destruct H. destruct H0. destruct H0.
+    assert (Hin :  (\bigcup_(x in lst) (semProdSizeOpt x x0)) a).
+    { eexists. split; eauto. }
+    eapply (@enumerate_correct_size_opt A) in Hin.
+    eexists. split; eauto. 
+Qed.       
+
